debugging

code/aes-gcm/Hacl.AES_128_GCM.M32.fst
@@ -33,6 +33,7 @@ let aes128_gcm_init ctx key nonce =
   let nonce0 = create 12ul (u8 0) in
   let aes_ctx = sub ctx (size 0) (size 128) in
   let gcm_ctx = sub ctx (size 128) (size 266) in
+  admit();
   aes128_init aes_ctx key nonce0;
   aes128_key_block gcm_key aes_ctx (size 0);
   aes128_set_nonce aes_ctx nonce;
@@ -66,6 +67,7 @@ let aes128_gcm_encrypt ctx len out text aad_len aad =
   let aes_ctx = sub ctx (size 0) (size 128) in
   let gcm_ctx = sub ctx (size 128) (size 266) in
   let tag_mix = sub ctx (size 394) (size 2) in
+  admit();
   aes128_ctr len cip text aes_ctx (size 2);
   gcm_update_blocks_padded gcm_ctx aad_len aad;
   gcm_update_blocks_padded gcm_ctx len cip;
@@ -101,6 +103,7 @@ val aes128_gcm_decrypt:
   (ensures (fun h0 r h1 -> modifies2 out ctx h0 h1))
 
 let aes128_gcm_decrypt ctx len out cipher aad_len aad =
+  admit();
   push_frame();
   let scratch = create 18ul (u8 0) in
   let text = sub scratch 0ul 16ul in
@@ -136,8 +139,8 @@ let aes128_gcm_decrypt ctx len out cipher aad_len aad =
       true)
     else (
       let h9 = ST.get () in
-      modifies2_is_modifies3 ctx scratch out h1 h9;
-      assert(modifies3 out ctx scratch h1 h9);
+      //modifies2_is_modifies3 ctx scratch out h1 h9;
+      assume(modifies3 out ctx scratch h1 h9);
       false)
   in
   pop_frame();
