code/aes/Hacl.Impl.AES.Core.fst
@@ -12,86 +12,86 @@ module ST = FStar.HyperStack.ST
 #set-options "--z3rlimit 50"
 
 
-inline_for_extraction
+inline_for_extraction noextract
 let create_state (#m:m_spec) =
   match m with
   | M32 -> Hacl.Impl.AES.CoreBitSlice.create_state()
   | MAES -> Hacl.Impl.AES.CoreNI.create_state()
 
-inline_for_extraction
+inline_for_extraction noextract
 let copy_state (#m:m_spec) (st:state m) (ost:state m) =
   match m with
   | MAES -> Hacl.Impl.AES.CoreNI.copy_state st ost
   | M32 -> Hacl.Impl.AES.CoreBitSlice.copy_state st ost
 
-inline_for_extraction
+inline_for_extraction noextract
 let load_block0 (#m:m_spec) (st:state m) (b:lbuffer uint8 16ul) =
   match m with
   | MAES -> Hacl.Impl.AES.CoreNI.load_block0 st b
   | M32 -> Hacl.Impl.AES.CoreBitSlice.load_block0 st b
 
-inline_for_extraction
+inline_for_extraction noextract
 let load_key1 (#m:m_spec) (k:key1 m) (b:lbuffer uint8 16ul) =
   match m with
   | MAES -> Hacl.Impl.AES.CoreNI.load_key1 k b
   | M32 -> Hacl.Impl.AES.CoreBitSlice.load_key1 k b
 
-inline_for_extraction
+inline_for_extraction noextract
 let load_nonce #m n b =
   match m with
   | MAES -> Hacl.Impl.AES.CoreNI.load_nonce n b
   | M32 -> Hacl.Impl.AES.CoreBitSlice.load_nonce n b
 
-inline_for_extraction
+inline_for_extraction noextract
 let load_state #m st n counter =
   match m with
   | MAES -> Hacl.Impl.AES.CoreNI.load_state st n counter
   | M32 -> Hacl.Impl.AES.CoreBitSlice.load_state st n counter
 
-inline_for_extraction
+inline_for_extraction noextract
 let store_block0 #m out st =
   match m with
   | MAES -> Hacl.Impl.AES.CoreNI.store_block0 out st
   | M32 -> Hacl.Impl.AES.CoreBitSlice.store_block0 out st
 
 
-inline_for_extraction
+inline_for_extraction noextract
 let xor_state_key1 #m st key =
   match m with
   | MAES -> Hacl.Impl.AES.CoreNI.xor_state_key1 st key
   | M32 -> Hacl.Impl.AES.CoreBitSlice.xor_state_key1 st key
 
-inline_for_extraction
+inline_for_extraction noextract
 let xor_block #m out st b =
   match m with
   | MAES -> Hacl.Impl.AES.CoreNI.xor_block out st b
   | M32 -> Hacl.Impl.AES.CoreBitSlice.xor_block out st b
 
-inline_for_extraction
+inline_for_extraction noextract
 let aes_enc #m st key =
   match m with
   | MAES -> Hacl.Impl.AES.CoreNI.aes_enc st key
   | M32 -> Hacl.Impl.AES.CoreBitSlice.aes_enc st key
 
-inline_for_extraction
+inline_for_extraction noextract
 let aes_enc_last #m st key =
   match m with
   | MAES -> Hacl.Impl.AES.CoreNI.aes_enc_last st key
   | M32 -> Hacl.Impl.AES.CoreBitSlice.aes_enc_last st key
 
-inline_for_extraction
+inline_for_extraction noextract
 let aes_keygen_assist0 #m n p rcon =
   match m with
   | MAES -> Hacl.Impl.AES.CoreNI.aes_keygen_assist0 n p rcon
   | M32 -> Hacl.Impl.AES.CoreBitSlice.aes_keygen_assist0 n p rcon
 
-inline_for_extraction
+inline_for_extraction noextract
 let aes_keygen_assist1 #m n p =
   match m with
   | MAES -> Hacl.Impl.AES.CoreNI.aes_keygen_assist1 n p
   | M32 -> Hacl.Impl.AES.CoreBitSlice.aes_keygen_assist1 n p
 
-inline_for_extraction
+inline_for_extraction noextract
 let key_expansion_step #m n p =
   match m with
   | MAES -> Hacl.Impl.AES.CoreNI.key_expansion_step n p
