code/aes/Hacl.Impl.AES.Core.fsti
@@ -14,47 +14,47 @@ type m_spec =
   | MAES
   | M32
 
-unfold
+unfold noextract
 let stelem (m:m_spec) =
   match m with
   | MAES -> vec_t U128 1
   | M32 -> uint64
 
-unfold
+unfold noextract
 let stlen (m:m_spec) =
   match m with
   | MAES -> 4ul
   | M32 -> 8ul
 
-unfold
+unfold noextract
 let klen (m:m_spec) =
   match m with
   | MAES -> 1ul
   | M32 -> 8ul
 
-unfold
+unfold noextract
 let nlen (m:m_spec) =
   match m with
   | MAES -> 1ul
   | M32 -> 8ul
 
-unfold
+unfold noextract
 let elem_zero (m:m_spec) : stelem m =
   match m with
   | M32 -> u64 0
   | MAES -> vec_zero U128 1
 
-unfold
+unfold noextract
 let state (m:m_spec) = lbuffer (stelem m) (stlen m)
 
-unfold
+unfold noextract
 let key1 (m:m_spec) = lbuffer (stelem m) (klen m)
 
-unfold
+unfold noextract
 let nonce (m:m_spec) = lbuffer (stelem m) (nlen m)
 
 
-inline_for_extraction
+inline_for_extraction noextract
 val create_state:
   #m: m_spec ->
   StackInline (state m)
@@ -62,7 +62,7 @@ val create_state:
   (ensures  (fun h0 f h1 -> live h1 f /\ stack_allocated f h0 h1 (Seq.create (v (stlen m)) (elem_zero m))))
 
 
-inline_for_extraction
+inline_for_extraction noextract
 val copy_state:
     #m: m_spec
   -> st: state m
@@ -71,7 +71,7 @@ val copy_state:
   (requires (fun h -> live h st /\ live h ost /\ disjoint st ost))
   (ensures  (fun h0 _ h1 -> modifies1 st h0 h1))
 
-inline_for_extraction
+inline_for_extraction noextract
 val load_block0:
     #m: m_spec
   -> st: state m
@@ -80,7 +80,7 @@ val load_block0:
   (requires (fun h -> live h st /\ live h b))
   (ensures  (fun h0 _ h1 -> modifies1 st h0 h1))
 
-inline_for_extraction
+inline_for_extraction noextract
 val load_key1:
     #m: m_spec
   -> k: key1 m
@@ -89,7 +89,7 @@ val load_key1:
   (requires (fun h -> live h k /\ live h b))
   (ensures  (fun h0 _ h1 -> modifies1 k h0 h1))
 
-inline_for_extraction
+inline_for_extraction noextract
 val load_nonce:
     #m: m_spec
   -> n: nonce m
@@ -98,7 +98,7 @@ val load_nonce:
   (requires (fun h -> live h n /\ live h b))
   (ensures  (fun h0 _ h1 -> modifies1 n h0 h1))
 
-inline_for_extraction
+inline_for_extraction noextract
 val load_state:
     #m: m_spec
   -> st: state m
@@ -108,7 +108,7 @@ val load_state:
   (requires (fun h -> live h st /\ live h nonce))
   (ensures  (fun h0 _ h1 -> modifies1 st h0 h1))
 
-inline_for_extraction
+inline_for_extraction noextract
 val store_block0:
     #m: m_spec
   -> out: lbuffer uint8 16ul
@@ -117,7 +117,7 @@ val store_block0:
   (requires (fun h -> live h st /\ live h out))
   (ensures  (fun h0 _ h1 -> modifies1 out h0 h1))
 
-inline_for_extraction
+inline_for_extraction noextract
 val xor_state_key1:
     #m: m_spec
   -> st: state m
@@ -126,7 +126,7 @@ val xor_state_key1:
   (requires (fun h -> live h st /\ live h key))
   (ensures  (fun h0 _ h1 -> modifies1 st h0 h1))
 
-inline_for_extraction
+inline_for_extraction noextract
 val xor_block:
     #m: m_spec
   -> out: lbuffer uint8 64ul
@@ -136,7 +136,7 @@ val xor_block:
   (requires (fun h -> live h st /\ live h out /\ live h b))
   (ensures  (fun h0 _ h1 -> modifies2 out st h0 h1))
 
-inline_for_extraction
+inline_for_extraction noextract
 val aes_enc:
     #m: m_spec
   -> st: state m
@@ -145,7 +145,7 @@ val aes_enc:
   (requires (fun h -> live h st /\ live h key))
   (ensures  (fun h0 _ h1 -> modifies1 st h0 h1))
 
-inline_for_extraction
+inline_for_extraction noextract
 val aes_enc_last:
     #m: m_spec
   -> st: state m
@@ -154,7 +154,7 @@ val aes_enc_last:
   (requires (fun h -> live h st /\ live h key))
   (ensures  (fun h0 _ h1 -> modifies1 st h0 h1))
 
-inline_for_extraction
+inline_for_extraction noextract
 val aes_keygen_assist0:
     #m: m_spec
   -> ok: key1 m
@@ -164,7 +164,7 @@ val aes_keygen_assist0:
   (requires (fun h -> live h ok /\ live h ik /\ disjoint ik ok))
   (ensures  (fun h0 _ h1 -> modifies1 ok h0 h1))
 
-inline_for_extraction
+inline_for_extraction noextract
 val aes_keygen_assist1:
     #m: m_spec
   -> ok: key1 m
@@ -173,7 +173,7 @@ val aes_keygen_assist1:
   (requires (fun h -> live h ok /\ live h ik /\ disjoint ik ok))
   (ensures  (fun h0 _ h1 -> modifies1 ok h0 h1))
 
-inline_for_extraction
+inline_for_extraction noextract
 val key_expansion_step:
     #m: m_spec
   -> next: key1 m
